theories/datatypes_properties.v
@@ -246,8 +246,7 @@ Canonical Structure module_export_desc_eqMixin := EqMixin eqmodule_export_descP.
 Canonical Structure module_export_desc_eqType := Eval hnf in EqType module_export_desc module_export_desc_eqMixin.
 
 Definition module_export_eq_dec : forall v1 v2 : module_export, {v1 = v2} + {v1 <> v2}.
-(* TODO: "decidable equality" diverges; why? *)
-Admitted. 
+Proof. decidable_equality. Defined.
 Definition module_export_eqb v1 v2 : bool := module_export_eq_dec v1 v2.
 Definition eqmodule_exportP : Equality.axiom module_export_eqb :=
   eq_dec_Equality_axiom module_export_eq_dec.
@@ -261,6 +260,14 @@ Definition administrative_instruction_rect' :=
 
 Definition administrative_instruction_ind' (P : administrative_instruction -> Prop) :=
   @administrative_instruction_rect' P.
+
+(** Administrative instructions frequently come in lists.
+  Here is the corresponding induction principle. **)
+Definition seq_administrative_instruction_rect' :=
+  ltac:(rect'_build_list administrative_instruction_rect).
+
+Definition seq_administrative_instruction_ind' (P : administrative_instruction -> Prop) :=
+  @seq_administrative_instruction_rect' P.
 
 Definition administrative_instruction_eq_dec : forall e1 e2 : administrative_instruction,
   {e1 = e2} + {e1 <> e2}.
