theories/type_checker_reflects_typing.v
@@ -19,8 +19,6 @@ Proof.
   rewrite subn0. apply/eqP. by apply drop_size.
 Qed.
 
-Print upd_local_label_return.
-
 Lemma upd_label_overwrite: forall C loc lab ret lab',
   upd_label (upd_local_label_return C loc lab ret) lab'
   = upd_local_label_return C loc lab' ret.
@@ -85,7 +83,6 @@ Proof.
     unfold cl_typing_self in tc_prop.
     inversion tc_prop; subst => //.
     clear H5.
-    Print be_typing_ind.
     clear tc_prop.
     
     dependent induction H2; try (inversion Heqtf; subst; clear Heqtf) => //.
